Define interp_ptstomem in proof mode

case_study/RiscvPmpBoundedInts/IrisInstance.v
@@ -101,14 +101,22 @@ Module RiscvPmpIrisInstance <:
       [∗ list] offset ∈ seq 0 width,
         interp_ptsto (addr + bv.of_nat offset) (get_byte offset bytes).
 
-    Fixpoint interp_ptstomem {width : nat} (addr : Addr) (bytes : bv (width * byte)) : iProp Σ :=
+    Fixpoint interp_ptstomem {width : nat} (addr : Addr) (bytes : bv (width * byte)) : iProp Σ.
+    Proof.
+      destruct width.
+      - exact True%I.
+      - destruct (bv.appView byte (width * byte) bytes) as [byte bytes].
+        exact (interp_ptsto addr byte ∗ interp_ptstomem width (bv.one xlenbits + addr) bytes)%I.
+        Show Proof.
+    Defined.
+
+    (* Fixpoint interp_ptstomem {width : nat} (addr : Addr) (bytes : bv (width * byte)) : iProp Σ :=
       match width with
       | O   => True
       | S w =>
-          let bytes : bv (byte + w * byte) := bytes in
           let (byte, bytes) := bv.appView byte (w * byte) bytes in
           interp_ptsto addr byte ∗ interp_ptstomem (bv.one xlenbits + addr) bytes
-      end.
+      end. *)
 
     Definition interp_pmp_addr_access (addrs : list Addr) (entries : list PmpEntryCfg) (m : Privilege) : iProp Σ :=
       [∗ list] a ∈ addrs,
